proves all properties for heq, including at l = sprop

theories/HEq.v
@@ -67,7 +67,24 @@ Parameter obseq_forall_2@{u v+} :
         (x : A'), 
         (B (obseq_forall_1 e # x)) ~ (B' x).
 
+Axiom obseq_forall_1_sprop : 
+    forall 
+        {A A' : SProp} 
+        {B : A -> Type} {B' : A' -> Type}, 
+        (forall (x : A), B x) ~ (forall (x : A'), B' x) -> 
+        A' ~ A.
+
+Parameter obseq_forall_2_sprop : 
+    forall 
+        {A A' : SProp} {B : A -> Type} {B' : A' -> Type}
+        (e : (forall (x : A), B x) ~ (forall (x : A'), B' x))
+        (x : A'), 
+        (B (obseq_forall_1_sprop e #% x)) ~ (B' x).
+
 Parameter funext : forall {A B} (f g : forall (x : A), B x), (forall (x : A), f x ~ g x) -> f ~ g.
+
+
+Parameter funext_sprop : forall {A : SProp} {B} (f g : forall (x : A), B x), (forall (x : A), f x ~ g x) -> f ~ g.
 
 Axiom cast_pi : forall A B A' B' e f, 
     cast (forall (x : A), B x) (forall (x : A'), B' x) e f 
@@ -75,6 +92,14 @@ Axiom cast_pi : forall A B A' B' e f,
                             (B' x)
                             (obseq_forall_2 e x)
                             (f (cast A' A (obseq_forall_1 e) x)).
+
+
+Axiom cast_pi_sprop : forall A B A' B' e f, 
+    cast (forall (x : A), B x) (forall (x : A'), B' x) e f 
+    ~ fun (x : A') => cast (B (cast_prop A' A (obseq_forall_1_sprop e) x))
+                            (B' x)
+                            (obseq_forall_2_sprop e x)
+                            (f (cast_prop A' A (obseq_forall_1_sprop e) x)).                    
 
 Parameter propext : forall {A B : SProp}, (A -> B) -> (B -> A) -> A ~ B.
 
@@ -86,6 +111,7 @@ Axiom Acc : forall (A : Type) (R : A -> A -> SProp) (a : A), SProp.
 Axiom acc_in : forall A R a (f : forall y, R a y -> Acc A R y), Acc A R a.
 Axiom acc_inv : forall A R a, Acc A R a -> forall b, R a b -> Acc A R b.
 Axiom acc_el : forall A R (P : A -> Type) (p : forall (a : A) (ϵf : forall y : A, R a y -> P y), P a) (y : A) (r : Acc A R y), P y.
+Axiom acc_el_prop : forall A R (P : A -> SProp) (p : forall (a : A) (ϵf : forall y : A, R a y -> P y), P a) (y : A) (r : Acc A R y), P y.
 (* end of Acc *)
 
 (* Constructing Sigmas *)
@@ -101,38 +127,21 @@ Definition snd {A B}: forall (x : Σ A B), B (fst x) :=
 Definition mkΣ {A B} (a : A) (b : B a) : Σ A B := 
     fun P f => f a b.
 
-(* the heterogeneous equality *)
-Definition heq (A B : Type) (a : A) (b : B) := 
+(* the heterogeneous equality at sort Type *)
+Definition heq_ty (A B : Type) (a : A) (b : B) := 
     Σ (A ~ B) (fun eq_ty => (eq_ty # a) ~ b).
 
-Notation "a == b" := (heq _ _ a b) (at level 90).
+Notation "a == b" := (heq_ty _ _ a b) (at level 90).
 
-Lemma heq_refl {A : Type} (a : A) : a == a. 
-Proof.
-    unfold heq. unshelve eapply mkΣ.
-    - eapply obseq_refl.
-    - eapply cast_refl.
-Qed.
 
-Lemma heq_sym {A B : Type} {a : A} {b : B} (e : a == b) : b == a. 
-Proof.
-    unshelve eapply mkΣ.
-    - eapply obseq_sym. eapply fst in e. assumption.
-    - unfold heq in e. eapply fst in e as e1. 
-      pose proof (e2 := snd e). simpl in e2.
-      destruct e1. destruct e2. eapply obseq_trans.
-      eapply cast_refl.
-      eapply cast_refl.
-Qed.
+Inductive True : SProp := I.
 
-Lemma heq_trans {A B C} {a : A} {b : B} {c : C} (p : a == b) (q : b == c) : a == c.
-Proof.
-    eapply fst in p as p1. pose proof (p2 := snd p).
-    eapply fst in q as q1. pose proof (q2 := snd q). simpl in p2,q2.
-    destruct p1. destruct q1. destruct q2. destruct p2.
-    unshelve eapply mkΣ. eapply obseq_refl.
-    eapply obseq_sym. eapply cast_refl.
-Qed.
+(* the heterogeneous equality at sort SProp *)
+Definition heq_prop (A B : SProp) (a : A) (b : B) : SProp := True.
+
+Notation "a ~~ b" := (heq_prop _ _ a b) (at level 90).
+
+(* auxiliary lemmas *)
 
 Lemma homo_to_hetero {A : Type} {a b : A} (e : a ~ b) : a == b.
 Proof.
@@ -146,44 +155,134 @@ Proof.
     destruct e1. destruct e2. eapply obseq_sym. eapply cast_refl.
 Qed.
 
-Lemma heq_cast {A B} {e : A ~ B} {a} : a == (e # a).
-Proof.
-    destruct e. 
-    eapply homo_to_hetero, obseq_sym, cast_refl.
-Qed.
-
-(* Definition cast_heq {A B : Type} (e : A == B) (a : A) : B := hetero_to_homo e # a. *)
-
 Lemma ap' {A B} (f g : forall x : A, B x) (t : A): f ~ g -> f t ~ g t.
 Proof.
     intros. destruct H. eapply obseq_refl.
 Qed.
 
-Lemma heq_app : forall {A1 A2 : Type} {B1 : A1 -> Type} {B2 : A2 -> Type} 
+
+Lemma ap_sprop' {A : SProp} {B} (f g : forall x : A, B x) (t : A): f ~ g -> f t ~ g t.
+Proof.
+    intros. destruct H. eapply obseq_refl.
+Qed.
+
+
+(* -- heq_refl -- *)
+
+Lemma heq_ty_refl {A : Type} (a : A) : a == a. 
+Proof.
+    unfold heq_ty. unshelve eapply mkΣ.
+    - eapply obseq_refl.
+    - eapply cast_refl.
+Qed.
+
+Lemma heq_prop_refl {A : SProp} (a : A) : a ~~ a.
+Proof.
+    econstructor.
+Qed.
+
+(* -- heq_sym -- *)
+
+Lemma heq_ty_sym {A B : Type} {a : A} {b : B} (e : a == b) : b == a. 
+Proof.
+    unshelve eapply mkΣ.
+    - eapply obseq_sym. eapply fst in e. assumption.
+    - unfold heq_ty in e. eapply fst in e as e1. 
+      pose proof (e2 := snd e). simpl in e2.
+      destruct e1. destruct e2. eapply obseq_trans.
+      eapply cast_refl.
+      eapply cast_refl.
+Qed.
+
+Lemma heq_prop_sym {A B : SProp} {a : A} {b : B} (e : a ~~ b) : b ~~ a. 
+Proof.
+    econstructor.
+Qed.
+
+(* -- heq_trans -- *)
+
+Lemma heq_ty_trans {A B C} {a : A} {b : B} {c : C} (p : a == b) (q : b == c) : a == c.
+Proof.
+    eapply fst in p as p1. pose proof (p2 := snd p).
+    eapply fst in q as q1. pose proof (q2 := snd q). simpl in p2,q2.
+    destruct p1. destruct q1. destruct q2. destruct p2.
+    unshelve eapply mkΣ. eapply obseq_refl.
+    eapply obseq_sym. eapply cast_refl.
+Qed.
+
+Lemma heq_prop_trans {A B C} {a : A} {b : B} {c : C} (p : a ~~ b) (q : b ~~ c) : a ~~ c.
+Proof.
+    econstructor.
+Qed.
+
+(* -- heq_cast -- *)
+
+Lemma heq_ty_cast {A B} {e : A ~ B} {a} : a == (e # a).
+Proof.
+    destruct e. 
+    eapply homo_to_hetero, obseq_sym, cast_refl.
+Qed.
+
+Lemma heq_prop_cast {A B} {e : A ~ B} {a} : a ~~ (e #% a).
+Proof.
+    econstructor.
+Qed.
+
+
+(* -- heq_app -- *)
+
+Lemma heq_ty_ty_app : forall {A1 A2 : Type} {B1 : A1 -> Type} {B2 : A2 -> Type} 
     {f : forall x : A1, B1 x} {g : forall x : A2, B2 x} {t : A1} {u : A2} (p : f == g) (q : t == u), (f t) == (g u).
 Proof.  
     intros.
     eapply fst in p as p1. pose proof (p2 := snd p).
     eapply fst in q as q1. pose proof (q2 := snd q). simpl in p2,q2.
     destruct q1. destruct q2.
-    unshelve eapply heq_trans.
+    unshelve eapply heq_ty_trans.
     2:exact (g t).
     - unshelve eapply mkΣ.
       * pose (e := obseq_forall_2 p1 t). destruct e. eapply ap. eapply obseq_sym, cast_refl.
       * destruct p2. eapply obseq_trans.
         2:eapply ap', obseq_sym, cast_pi.
         simpl. eapply hetero_to_homo. 
-        eapply heq_trans. eapply heq_sym, heq_cast.
-        eapply heq_trans. 2:eapply heq_cast.
+        eapply heq_ty_trans. eapply heq_ty_sym, heq_ty_cast.
+        eapply heq_ty_trans. 2:eapply heq_ty_cast.
         pose proof (e := cast_refl _ (obseq_forall_1 (fst p)) t).
         unshelve eapply (obseq_sind _ _ (fun t' _ => f t' == f (cast A1 A1 (obseq_forall_1 (fst p)) t)) _ _).
-        2:eapply heq_refl. eapply cast_refl.
+        2:eapply heq_ty_refl. eapply cast_refl.
     - unshelve eapply (obseq_sind _ _ (fun t' _ => g t' == g (cast A1 A1 (fst q) t)) _ _).
-      2:eapply heq_refl. eapply cast_refl.
+      2:eapply heq_ty_refl. eapply cast_refl.
 Qed.
 
+Lemma heq_prop_ty_app : forall {A1 A2 : SProp} {B1 : A1 -> Type} {B2 : A2 -> Type} 
+    {f : forall x : A1, B1 x} {g : forall x : A2, B2 x} {t : A1} {u : A2} (p : f == g) (q : t ~~ u), (f t) == (g u).
+Proof.
+    intros.
+    eapply fst in p as p1. pose proof (p2 := snd p). simpl in p2.
+    pose (e1 := obseq_forall_1_sprop p1). destruct e1.
+    unshelve eapply mkΣ.
+      * pose (e := obseq_forall_2_sprop p1 t). eapply e.
+      * destruct p2. eapply obseq_trans.
+        2:eapply ap_sprop', obseq_sym, cast_pi_sprop.
+        reflexivity.
+Qed.
 
-Definition heq_funext : forall {A : Type} {B1 B2 : A -> Type} {f : forall x : A, B1 x} {g : forall x : A, B2 x} (p : forall x, f x == g x), f == g.
+Lemma heq_ty_prop_app : forall {A1 A2 : Type} {B1 : A1 -> SProp} {B2 : A2 -> SProp} 
+    {f : forall x : A1, B1 x} {g : forall x : A2, B2 x} {t : A1} {u : A2} (p : f ~~ g) (q : t == u), (f t) ~~ (g u).
+Proof.
+    intros.
+    econstructor.
+Qed.
+
+Lemma heq_prop_prop_app : forall {A1 A2 : SProp} {B1 : A1 -> SProp} {B2 : A2 -> SProp} 
+    {f : forall x : A1, B1 x} {g : forall x : A2, B2 x} {t : A1} {u : A2} (p : f ~~ g) (q : t ~~ u), (f t) ~~ (g u).
+Proof.
+    intros. econstructor.
+Qed.
+
+(* more auxiliary lemmas *)
+
+Definition heq_ty_ty_funext : forall {A : Type} {B1 B2 : A -> Type} {f : forall x : A, B1 x} {g : forall x : A, B2 x} (p : forall x, f x == g x), f == g.
 Proof.
     intros. unshelve eapply mkΣ.
     - eapply (ap (fun B => forall x : A, B x)). 
@@ -195,25 +294,45 @@ Proof.
       destruct px2. eapply obseq_trans.
       eapply ap'. eapply cast_pi. simpl.
       eapply hetero_to_homo.
-      eapply heq_trans.
-      eapply heq_sym, heq_cast.
-      eapply heq_trans. 2:eapply heq_cast.
-      eapply heq_app. eapply heq_refl. eapply homo_to_hetero, cast_refl.
+      eapply heq_ty_trans.
+      eapply heq_ty_sym, heq_ty_cast.
+      eapply heq_ty_trans. 2:eapply heq_ty_cast.
+      eapply heq_ty_ty_app. eapply heq_ty_refl. eapply homo_to_hetero, cast_refl.
 Qed.
 
-Definition heq_funext' {A1 A2 : Type} {B1 : A1 -> Type} {B2 : A2 -> Type} 
+
+Definition heq_sprop_ty_funext : forall {A : SProp} {B1 B2 : A -> Type} {f : forall x : A, B1 x} {g : forall x : A, B2 x} (p : forall x, f x == g x), f == g.
+Proof.
+    intros. unshelve eapply mkΣ.
+    - eapply (ap (fun B => forall x : A, B x)). 
+      eapply funext_sprop. intros. pose proof (px := p x).
+      pose (px1 := fst px). assumption.
+    - eapply funext_sprop. intros.
+      pose proof (px := p x).
+      pose (px1 := fst px). pose (px2 := snd px). simpl in px2.
+      destruct px2. eapply obseq_trans.
+      eapply ap_sprop'. eapply cast_pi_sprop. simpl.
+      eapply hetero_to_homo.
+      eapply heq_ty_trans.
+      eapply heq_ty_sym. 
+      eapply (@heq_ty_cast (B1 (cast_prop A A (obseq_forall_1_sprop (ap (fun B : A -> Type => forall x0 : A, B x0) (funext_sprop B1 B2 (fun x0 : A => fst (p x0))))) x)) (B2 x)).
+      eapply heq_ty_trans. 2:eapply heq_ty_cast. eapply heq_ty_refl.
+Qed.
+
+Definition heq_ty_ty_funext' {A1 A2 : Type} {B1 : A1 -> Type} {B2 : A2 -> Type} 
     {f : forall x : A1, B1 x} {g : forall x : A2, B2 x} (e : A1 ~ A2) (p : forall x, f x == g (e # x)) : f == g.   
 Proof.
     destruct e.
-    eapply heq_funext.
+    eapply heq_ty_ty_funext.
     intros.
-    eapply heq_trans.
+    eapply heq_ty_trans.
     exact (p x).
-    eapply heq_app. eapply heq_refl. eapply homo_to_hetero, cast_refl.
+    eapply heq_ty_ty_app. eapply heq_ty_refl. eapply homo_to_hetero, cast_refl.
 Qed.
 
+(* -- heq_pi -- *)
 
-Lemma heq_pi {A1 A2 : Type} {B1 : A1 -> Type} {B2 : A2 -> Type} (e1 : A1 == A2) (e2 : forall x1 x2, x1 == x2 -> B1 x1 == B2 x2) 
+Lemma heq_ty_ty_pi {A1 A2 : Type} {B1 : A1 -> Type} {B2 : A2 -> Type} (e1 : A1 == A2) (e2 : forall x1 x2, x1 == x2 -> B1 x1 == B2 x2) 
     : (forall x : A1, B1 x) == (forall x : A2, B2 x).
 Proof.
     eapply hetero_to_homo in e1. destruct e1. 
@@ -221,56 +340,147 @@ Proof.
     eapply (ap (fun B => forall x : A1, B x)).
     eapply funext. intros.
     eapply hetero_to_homo.
-    eapply e2. eapply heq_refl.
+    eapply e2. eapply heq_ty_refl.
 Qed.
 
-Lemma heq_lam {A1 A2 : Type} {B1 : A1 -> Type} {B2 : A2 -> Type} 
+
+Lemma heq_sprop_ty_pi {A1 A2 : SProp} {B1 : A1 -> Type} {B2 : A2 -> Type} (e1 : A1 == A2) (e2 : forall x1 x2, x1 ~~ x2 -> B1 x1 == B2 x2) 
+    : (forall x : A1, B1 x) == (forall x : A2, B2 x).
+Proof.
+    eapply hetero_to_homo in e1. destruct e1. 
+    eapply homo_to_hetero.
+    eapply (ap (fun B => forall x : A1, B x)).
+    eapply funext_sprop. intros.
+    eapply hetero_to_homo.
+    eapply e2. econstructor.
+Qed.
+
+Lemma heq_ty_sprop_pi {A1 A2 : Type} {B1 : A1 -> SProp} {B2 : A2 -> SProp} (e1 : A1 == A2) (e2 : forall x1 x2, x1 == x2 -> B1 x1 == B2 x2) 
+    : (forall x : A1, B1 x) == (forall x : A2, B2 x).
+Proof.
+    eapply hetero_to_homo in e1. destruct e1. 
+    eapply homo_to_hetero.
+    eapply (ap (fun B => forall x : A1, B x)).
+    eapply funext. intros.
+    eapply hetero_to_homo.
+    eapply e2. eapply heq_ty_refl.
+Qed.
+
+Lemma heq_sprop_sprop_pi {A1 A2 : SProp} {B1 : A1 -> SProp} {B2 : A2 -> SProp} (e1 : A1 == A2) (e2 : forall x1 x2, x1 ~~ x2 -> B1 x1 == B2 x2) 
+    : (forall x : A1, B1 x) == (forall x : A2, B2 x).
+Proof.
+    eapply hetero_to_homo in e1. destruct e1. 
+    eapply homo_to_hetero.
+    eapply (ap (fun B => forall x : A1, B x)).
+    eapply funext_sprop. intros.
+    eapply hetero_to_homo.
+    eapply e2. econstructor.
+Qed.
+
+(* -- heq_lam -- *)
+
+Lemma heq_ty_ty_lam {A1 A2 : Type} {B1 : A1 -> Type} {B2 : A2 -> Type} 
     {f1 : forall x : A1, B1 x} {f2 : forall x : A2, B2 x} 
     (e1 : A1 == A2) (e2 : forall x1 x2, x1 == x2 -> f1 x1 == f2 x2) 
     : (fun x => f1 x) == (fun x => f2 x).
 Proof.
     eapply hetero_to_homo in e1. destruct e1.
-    eapply heq_funext. intros.
-    eapply e2. eapply heq_refl.
+    eapply heq_ty_ty_funext. intros.
+    eapply e2. eapply heq_ty_refl.
 Qed.
 
+
+Lemma heq_sprop_ty_lam {A1 A2 : SProp} {B1 : A1 -> Type} {B2 : A2 -> Type} 
+    {f1 : forall x : A1, B1 x} {f2 : forall x : A2, B2 x} 
+    (e1 : A1 == A2) (e2 : forall x1 x2, x1 ~~ x2 -> f1 x1 == f2 x2) 
+    : (fun x => f1 x) == (fun x => f2 x).
+Proof.
+    eapply hetero_to_homo in e1. destruct e1.
+    eapply heq_sprop_ty_funext. intros.
+    eapply e2. econstructor.
+Qed.
+
+Lemma heq_ty_sprop_lam {A1 A2 : Type} {B1 : A1 -> SProp} {B2 : A2 -> SProp} 
+    {f1 : forall x : A1, B1 x} {f2 : forall x : A2, B2 x} 
+    (e1 : A1 == A2) (e2 : forall x1 x2, x1 == x2 -> f1 x1 ~~ f2 x2) 
+    : (fun x => f1 x) ~~ (fun x => f2 x).
+Proof.
+    intros. econstructor.
+Qed.
+
+Lemma heq_sprop_sprop_lam {A1 A2 : SProp} {B1 : A1 -> SProp} {B2 : A2 -> SProp} 
+    {f1 : forall x : A1, B1 x} {f2 : forall x : A2, B2 x} 
+    (e1 : A1 == A2) (e2 : forall x1 x2, x1 ~~ x2 -> f1 x1 ~~ f2 x2) 
+    : (fun x => f1 x) ~~ (fun x => f2 x).
+Proof.
+    intros. econstructor.
+Qed.
+
+(* -- heq_obseq -- *)
 
 Lemma heq_obseq {A1 A2 : Type} {a1 b1 : A1} {a2 b2 : A2} 
     (e2 : a1 == a2) (e3 : b1 == b2) : (@obseq A1 a1 b1) == (@obseq A2 a2 b2).
 Proof.
     pose proof (e21 := fst e2). destruct e21.
     eapply hetero_to_homo in e2, e3. destruct e2, e3.
-    eapply heq_refl.
+    eapply heq_ty_refl.
 Qed.
 
-Lemma heq_natrec {P1 P2 : nat -> Type} {pzero1 : P1 O} {pzero2 : P2 O} 
+(* -- heq_succ -- *)
+
+Lemma heq_succ n m : n == m -> S n == S m.
+Proof.
+    intros. eapply hetero_to_homo in H. destruct H. eapply heq_ty_refl.
+Qed.
+
+(* -- heq_natrec -- *)
+
+Lemma heq_ty_natrec {P1 P2 : nat -> Type} {pzero1 : P1 O} {pzero2 : P2 O} 
         {psucc1 : forall x : nat, P1 x -> P1 (S x)} {psucc2 : forall x : nat, P2 x -> P2 (S x)} {n1 n2}
-        (e1 : forall x, P1 x == P2 x) (e2 : pzero1 == pzero2) 
-        (e3 : forall x p1 p2, p1 == p2 -> psucc1 x p1 == psucc2 x p2) 
+        (e1 : forall x1 x2, x1 == x2 -> P1 x1 == P2 x2) (e2 : pzero1 == pzero2) 
+        (e3 : forall x1 x2 p1 p2, x1 == x2 -> p1 == p2 -> psucc1 x1 p1 == psucc2 x2 p2) 
         (e4 : n1 == n2) : (@nat_rect P1 pzero1 psucc1 n1) == (@nat_rect P2 pzero2 psucc2 n2).
 Proof.
-    eapply heq_app; eauto.
-    eapply (@heq_app _ _ _ _ (nat_rect P1 pzero1) (nat_rect P2 pzero2)).
-    eapply (@heq_app _ _ _ _ (nat_rect P1) (nat_rect P2)).
-    eapply (@heq_app _ _ _ _ nat_rect nat_rect).
-    eapply heq_refl.
-    eapply heq_funext. eapply e1.
+    eapply heq_ty_ty_app; eauto.
+    eapply (@heq_ty_ty_app _ _ _ _ (nat_rect P1 pzero1) (nat_rect P2 pzero2)).
+    eapply (@heq_ty_ty_app _ _ _ _ (nat_rect P1) (nat_rect P2)).
+    eapply (@heq_ty_ty_app _ _ _ _ nat_rect nat_rect).
+    eapply heq_ty_refl.
+    eapply heq_ty_ty_funext. intros. eapply (e1 x x). eapply heq_ty_refl.
     eapply e2.
-    eapply heq_funext. intros.
-    unshelve eapply heq_funext'. 
-    2:{ intros. eapply e3. eapply heq_cast. }
-    eapply hetero_to_homo. eapply e1.
+    eapply heq_ty_ty_funext. intros.
+    unshelve eapply heq_ty_ty_funext'.
+    2:{ intros. eapply (e3 x x x0 _). eapply heq_ty_refl. eapply heq_ty_cast. }
+    eapply hetero_to_homo. eapply e1. eapply heq_ty_refl. 
 Qed.
 
-Lemma heq_cast' {A1 A2 B1 B2} (e1 : A1 ~ B1) (e2 : A2 ~ B2) (a1 : A1) (a2 : A2) (e : a1 == a2) : (e1 # a1) == (e2 # a2).
+Lemma heq_sprop_natrec {P1 P2 : nat -> SProp} {pzero1 : P1 O} {pzero2 : P2 O} 
+        {psucc1 : forall x : nat, P1 x -> P1 (S x)} {psucc2 : forall x : nat, P2 x -> P2 (S x)} {n1 n2}
+        (e1 : forall x1 x2, x1 == x2 -> P1 x1 == P2 x2) (e2 : pzero1 ~~ pzero2) 
+        (e3 : forall x1 x2 p1 p2, x1 == x2 -> p1 ~~ p2 -> psucc1 x1 p1 ~~ psucc2 x2 p2) 
+        (e4 : n1 == n2) : (@nat_sind P1 pzero1 psucc1 n1) ~~ (@nat_sind P2 pzero2 psucc2 n2).
+Proof.
+    econstructor.
+Qed.
+
+(* -- heq_cast' -- *)
+
+Lemma heq_ty_cast' {A1 A2 B1 B2} (e1 : A1 ~ B1) (e2 : A2 ~ B2) (a1 : A1) (a2 : A2) (e : a1 == a2) : (e1 # a1) == (e2 # a2).
 Proof.
     destruct e1. destruct e2. 
     pose proof (e1 := fst e). destruct e1.
-    eapply heq_trans. eapply heq_trans.
+    eapply heq_ty_trans. eapply heq_ty_trans.
     2:exact e.
-    eapply heq_sym. eapply (@heq_cast _ _ obseq_refl a1).
-    eapply heq_cast.
+    eapply heq_ty_sym. eapply (@heq_ty_cast _ _ obseq_refl a1).
+    eapply heq_ty_cast.
 Qed.
+
+Lemma heq_prop_cast' {A1 A2 B1 B2 : SProp} (e1 : A1 ~ B1) (e2 : A2 ~ B2) (a1 : A1) (a2 : A2) (e : a1 ~~ a2) : (e1 #% a1) ~~ (e2 #% a2).
+Proof.
+    econstructor.
+Qed.
+
+(* -- heq_acc -- *)
 
 Lemma heq_acc {A1 A2 R1 R2 a1 a2} 
         (e1 : forall x1 x2, x1 == x2 -> forall y1 y2, y1 == y2 -> R1 x1 y1 == R2 x2 y2) 
@@ -278,16 +488,18 @@ Lemma heq_acc {A1 A2 R1 R2 a1 a2}
         : (Acc A1 R1 a1) == (Acc A2 R2 a2).
 Proof.
     pose proof (e21 := fst e2). destruct e21.
-    eapply (@heq_app _ _ _ _ (Acc A1 R1) (Acc A1 R2)).
+    eapply (@heq_ty_ty_app _ _ _ _ (Acc A1 R1) (Acc A1 R2)).
     2:assumption.
-    eapply (@heq_app _ _ _ _ (Acc A1) (Acc A1)).
-    eapply heq_refl.
-    eapply heq_funext. intros.
-    eapply heq_funext. intros.
-    eapply e1; eauto using heq_refl.
+    eapply (@heq_ty_ty_app _ _ _ _ (Acc A1) (Acc A1)).
+    eapply heq_ty_refl.
+    eapply heq_ty_ty_funext. intros.
+    eapply heq_ty_ty_funext. intros.
+    eapply e1; eauto using heq_ty_refl.
 Qed.
 
-Lemma heq_acc_el {A1 A2 R1 R2 a1 a2 P1 P2 p1 p2}
+(* -- heq_acc_el -- *)
+
+Lemma heq_ty_acc_el {A1 A2 R1 R2 a1 a2 P1 P2 p1 p2}
     (e0 : forall x1 x2, x1 == x2 -> forall y1 y2, y1 == y2 -> R1 x1 y1 == R2 x2 y2) 
     (e1 : forall x1 x2, x1 == x2 -> P1 x1 == P2 x2)
     (e2 : forall x1 x2, x1 == x2 -> forall y1 y2, y1 == y2 -> p1 x1 y1 == p2 x2 y2)
@@ -295,28 +507,38 @@ Lemma heq_acc_el {A1 A2 R1 R2 a1 a2 P1 P2 p1 p2}
     : (acc_el A1 R1 P1 p1 a1) == (acc_el A2 R2 P2 p2 a2).
 Proof.
     pose proof (e31 := fst e3). destruct e31.
-    eapply (@heq_app _ _ _ _ (acc_el A1 R1 P1 p1) (acc_el A1 R2 P2 p2)).
+    eapply (@heq_ty_ty_app _ _ _ _ (acc_el A1 R1 P1 p1) (acc_el A1 R2 P2 p2)).
     2:assumption.
-    eapply (@heq_app _ _ _ _ (acc_el A1 R1 P1) (acc_el A1 R2 P2)).
-    eapply (@heq_app _ _ _ _ (acc_el A1 R1) (acc_el A1 R2)).
-    eapply (@heq_app _ _ _ _ (acc_el A1) (acc_el A1)).
-    eapply heq_refl.
-    eapply heq_funext. intros.
-    eapply heq_funext. intros.
-    eapply e0; eauto using heq_refl.
-    eapply heq_funext. intros. eapply e1; eauto using heq_refl.
-    eapply heq_funext. intros.
-    unshelve eapply heq_funext'. 
+    eapply (@heq_ty_ty_app _ _ _ _ (acc_el A1 R1 P1) (acc_el A1 R2 P2)).
+    eapply (@heq_ty_ty_app _ _ _ _ (acc_el A1 R1) (acc_el A1 R2)).
+    eapply (@heq_ty_ty_app _ _ _ _ (acc_el A1) (acc_el A1)).
+    eapply heq_ty_refl.
+    eapply heq_ty_ty_funext. intros.
+    eapply heq_ty_ty_funext. intros.
+    eapply e0; eauto using heq_ty_refl.
+    eapply heq_ty_ty_funext. intros. eapply e1; eauto using heq_ty_refl.
+    eapply heq_ty_ty_funext. intros.
+    unshelve eapply heq_ty_ty_funext'. 
     2:{intros.
-    eapply e2; eauto using heq_refl.
-    eapply heq_cast. }
+    eapply e2; eauto using heq_ty_refl.
+    eapply heq_ty_cast. }
     eapply (ap (fun B => forall x : A1, B x)).
     eapply hetero_to_homo.
-    eapply heq_funext.
+    eapply heq_ty_ty_funext.
     intros.
-    pose proof (e0' := e0 x x (heq_refl _) x0 x0 (heq_refl _)). 
+    pose proof (e0' := e0 x x (heq_ty_refl _) x0 x0 (heq_ty_refl _)). 
     eapply hetero_to_homo in e0'. destruct e0'.
-    pose proof (e1' := e1 x0 x0 (heq_refl _)).
+    pose proof (e1' := e1 x0 x0 (heq_ty_refl _)).
     eapply hetero_to_homo in e1'. destruct e1'.
-    eapply heq_refl.
+    eapply heq_ty_refl.
+Qed.
+
+Lemma heq_prop_acc_el {A1 A2 R1 R2 a1 a2} {P1 : A1 -> SProp} {P2 : A2 -> SProp} {p1 p2}
+    (e0 : forall x1 x2, x1 == x2 -> forall y1 y2, y1 == y2 -> R1 x1 y1 == R2 x2 y2) 
+    (e1 : forall x1 x2, x1 == x2 -> P1 x1 == P2 x2)
+    (e2 : forall x1 x2, x1 == x2 -> forall y1 y2, y1 ~~ y2 -> p1 x1 y1 ~~ p2 x2 y2)
+    (e3 : a1 == a2)
+    : (acc_el_prop A1 R1 P1 p1 a1) ~~ (acc_el_prop A2 R2 P2 p2 a2).
+Proof.
+    econstructor.
 Qed.
